lambda2Gmu/Regularity.v
@@ -6,45 +6,6 @@ Require Import TLC.LibLN.
 Require Import TLC.LibEnv.
 
 
-Ltac fold_delta :=
-  repeat match goal with
-  | [ H: context [List.map tc_var ?As] |- _ ] =>
-    fold (tc_vars As) in H
-  | [ H: context [ (tc_var ?X) :: ?As] |- _ ] =>
-    match As with
-    | []* => fail 1
-    | _ => fold ([tc_var X]* ++ As) in H
-    end
-  | [ H: context [ (tc_eq ?eq) :: ?As] |- _ ] =>
-    match As with
-    | []* => fail 1
-    | _ => fold ([tc_eq eq]* ++ As) in H
-    end
-  | [ |- context [List.map tc_var ?As] ] =>
-    fold (tc_vars As)
-  | [ |- context [ (tc_var ?X) :: ?As] ] =>
-    match As with
-    | []* => fail 1
-    | _ => fold ([tc_var X]* ++ As)
-    end
-  | [ |- context [ (tc_eq ?eq) :: ?As] ] =>
-    match As with
-    | []* => fail 1
-    | _ => fold ([tc_eq eq]* ++ As)
-    end
-  end.
-
-Ltac destruct_in_app :=
-  match goal with
-  | [ H: List.In ?X (?A ++ ?B) |- _ ] =>
-    apply List.in_app_or in H;
-    destruct H
-  | [ H: is_var_defined (?A ++ ?B) ?X |- _ ] =>
-    unfold is_var_defined in H;
-    apply List.in_app_or in H;
-    destruct H
-  end.
-
 (** * Regularity *)
 (**
 Defines basic properties of well formed types and typing judgement.
